cava/arrow-examples/ArrowExtraction.v
@@ -35,3 +35,15 @@ Extraction Library Mux2_1.
 Extraction Library UnsignedAdder.
 
 Extraction Library ArrowAdderTutorial.
+
+From Cava Require Import Arrow.ArrowExport.
+(* From Cava Require Import Cava.pkg. *)
+Extraction Library CavaNotation.
+Require Import Aes.pkg.
+Extraction Library pkg.
+Require Import Aes.sbox.
+Extraction Library sbox.
+Require Import Aes.sbox_canright_pkg.
+Extraction Library sbox_canright_pkg.
+Require Import Aes.sbox_canright.
+Extraction Library sbox_canright.
